src/program_proof/wal/write_proof.v
@@ -17,6 +17,67 @@ Context (P: log_state.t -> iProp Σ).
 Let N := walN.
 Let circN := walN .@ "circ".
 
+Definition memEnd (σ: locked_state): Z :=
+  int.val σ.(memStart) + length σ.(memLog).
+
+Hint Unfold locked_wf : word.
+Hint Unfold memEnd : word.
+
+Theorem wp_WalogState__updatesOverflowU64 st σ (newUpdates: u64) :
+  {{{ wal_linv_fields st σ }}}
+    WalogState__updatesOverflowU64 #st #newUpdates
+  {{{ (overflow:bool), RET #overflow; ⌜overflow = bool_decide (memEnd σ + int.val newUpdates >= 2^64)⌝ ∗
+                                      wal_linv_fields st σ
+  }}}.
+Proof.
+  iIntros (Φ) "Hfields HΦ".
+  iNamed "Hfields".
+  iNamed "Hfield_ptsto".
+  iDestruct (updates_slice_len with "His_memLog") as %HmemLog_sz.
+  wp_call.
+  rewrite /WalogState__memEnd.
+  wp_loadField. wp_loadField.
+  wp_apply wp_slice_len.
+  wp_apply util_proof.wp_SumOverflows.
+  iIntros (?) "->".
+  iApply "HΦ".
+  iSplit.
+  { iPureIntro.
+    apply bool_decide_iff.
+    word. }
+  iFrame.
+  iExists _; by iFrame.
+Qed.
+
+Theorem wp_WalogState__memLogHasSpace st σ (newUpdates: u64) :
+  memEnd σ + int.val newUpdates < 2^64 ->
+  {{{ wal_linv_fields st σ }}}
+    WalogState__memLogHasSpace #st #newUpdates
+  {{{ (has_space:bool), RET #has_space; ⌜has_space = bool_decide (memEnd σ - int.val σ.(diskEnd) + int.val newUpdates ≤ LogSz)⌝ ∗
+                                        wal_linv_fields st σ
+  }}}.
+Proof.
+  iIntros (Hnon_overflow Φ) "Hfields HΦ".
+  iNamed "Hfields".
+  iNamed "Hfield_ptsto".
+  iDestruct (updates_slice_len with "His_memLog") as %HmemLog_sz.
+  wp_call.
+  rewrite /WalogState__memEnd.
+  wp_loadField. wp_loadField.
+  wp_apply wp_slice_len.
+  wp_loadField.
+  wp_pures.
+  change (int.val $ word.divu (word.sub 4096 8) 8) with LogSz.
+  iAssert (wal_linv_fields st σ) with "[-HΦ]" as "Hfields".
+  { iFrame.
+    iExists _; by iFrame. }
+  wp_if_destruct; iApply "HΦ"; iFrame; iPureIntro.
+  - symmetry; apply bool_decide_eq_false.
+    revert Heqb; repeat word_cleanup.
+  - symmetry; apply bool_decide_eq_true.
+    revert Heqb; repeat word_cleanup.
+Qed.
+
 Theorem wp_Walog__MemAppend (PreQ : iProp Σ) (Q: u64 -> iProp Σ) l γ bufs bs :
   {{{ is_wal P l γ ∗
        updates_slice bufs bs ∗
@@ -46,6 +107,7 @@ Proof.
     iNamed "Hstfields".
     wp_loadField.
     wp_apply (acquire_spec with "lk"); iIntros "(Hlocked&Hlockinv)".
+    wp_loadField.
     wp_pures.
     wp_bind (For _ _ _).
     wp_apply (wp_forBreak_cond
@@ -68,28 +130,25 @@ Proof.
     { clear Φ.
       iIntros "!>" (Φ) "HI HΦ". iNamed "HI".
       wp_pures.
-      iNamed "Hlockinv".
-      iNamed "Hfields".
-      iNamed "Hfield_ptsto".
       wp_apply wp_slice_len.
-      wp_loadField. wp_loadField.
-      wp_apply util_proof.wp_SumOverflows.
-      iIntros "%->".
+      iNamed "Hlockinv".
+      wp_apply (wp_WalogState__updatesOverflowU64 with "Hfields").
+      iIntros (?) "[-> Hfields]".
+      wp_pures.
       wp_if_destruct.
       - wp_store.
+        wp_pures.
         iApply "HΦ".
         iExists _, _; iFrame.
         iDestruct "Hsim" as "[_ $]".
         iExists _; iFrame "# ∗".
-        iExists _; iFrame "# ∗".
-      - rewrite /WalogState__memEnd.
-        wp_loadField. wp_loadField. wp_loadField.
-        wp_apply wp_slice_len.
-        wp_loadField. wp_loadField.
-        iDestruct (updates_slice_len with "His_memLog") as %HmemLog_sz.
-        wp_apply wp_slice_len.
-        wp_pures.
+      - wp_apply wp_slice_len.
+        wp_apply (wp_WalogState__memLogHasSpace with "Hfields"); first by word.
+        iIntros (?) "[-> Hfields]".
         wp_if_destruct.
+        + admit.
         + wp_apply util_proof.wp_DPrintf.
-          wp_loadField.
+          admit.
 Abort.
+
+End goose_lang.
